add: signals and utils file

source/PriorityQueue.dfy
@@ -1,80 +1,6 @@
 include "Signal.dfy"
 include "Queue.dfy"
-
-function emptyLists<T>(size : nat) : seq<seq<T>>
-	ensures |emptyLists<T>(size)| == size
-	ensures forall i :: 0 <= i < size ==> emptyLists<T>(size)[i] == []
-	ensures flatten<T>(emptyLists<T>(size)) == []
-{
-	if size == 0 then
-		[]
-	else
-		[[]] + emptyLists(size - 1)
-}
-
-function flatten<T>(sequences : seq<seq<T>>) : seq<T>
-{
-	if |sequences| == 0 then
-		[]
-	else
-		sequences[0] + flatten(sequences[1..])
-}
-
-function firstNonEmpty<T>(sequences : seq<seq<T>>) : nat
-	requires flatten<T>(sequences) != []
-	ensures 0 <= firstNonEmpty<T>(sequences) < |sequences|
-	ensures |sequences[firstNonEmpty<T>(sequences)]| > 0
-	ensures forall k :: 0 <= k < |sequences| && sequences[k] != []
-	==> firstNonEmpty<T>(sequences) <= k
-{
-	if sequences[0] != [] then
-		0
-	else
-		1 + firstNonEmpty(sequences[1..])
-}
-
-function addTo<T>(sequences : seq<seq<T>>, priority : nat, value : T) : seq<seq<T>>
-	requires 0 < priority <= |sequences|
-	ensures |addTo(sequences, priority, value)| == |sequences|
-	ensures |flatten(addTo(sequences, priority, value))| == |flatten(sequences)| + 1
-	ensures forall i :: 0 <= i < |sequences| && i != index(priority) ==> addTo(sequences, priority, value)[i] == sequences[i]
-	ensures addTo(sequences, priority, value)[index(priority)] == sequences[index(priority)] + [value] 
-{
-	var changeIndex := index(priority);
-	if changeIndex == 0 then
-		[sequences[0] + [value]] + sequences[1..]
-	else
-		[sequences[0]] + addTo(sequences[1..], priority - 1, value)
-}
-
-function removeFrom<T>(sequences : seq<seq<T>>, priority : nat) : seq<seq<T>>
-	requires 0 < priority <= |sequences|
-	requires |sequences[index(priority)]| > 0 
-	ensures |removeFrom(sequences, priority)| == |sequences|
-	ensures |flatten(removeFrom(sequences, priority))| == |flatten(sequences)| - 1
-	ensures forall i :: 0 <= i < |sequences| && i != index(priority) ==> removeFrom(sequences, priority)[i] == sequences[i]
-	ensures removeFrom(sequences, priority)[index(priority)] == sequences[index(priority)][1..]
-{
-	var changeIndex := index(priority);
-	if changeIndex == 0 then
-		[sequences[0][1..]] + sequences[1..]
-	else
-		[sequences[0]] + removeFrom(sequences[1..], priority - 1)
-}
-
-function method index(priority : nat) : nat
-	requires 0 < priority
-	ensures 0 <= index(priority)
-{
-	priority - 1
-}
-
-function priority(index : nat) : nat
-	ensures 0 < priority(index)
-{
-	index + 1
-}
-
+include "Utils.dfy"
 
 class {:autocontracts} PriorityQueue
 {
@@ -112,12 +38,6 @@ class {:autocontracts} PriorityQueue
 		queues := queuesI;
 		this.elements := 0;
 		this.sequences := emptyLists(maxPriority);
-		// assert |sequences| == maxPriority;
-		// assert elements == |flatten(sequences)|;
-		// assert forall i :: 0 <= i < maxPriority ==> queues[i].Valid();
-		// assert forall i, j :: 0 <= i < j < maxPriority ==> queues[i] != queues[j];
-		// assert forall i :: 0 <= i < maxPriority ==> sequences[i] == queues[i].elemSeq;
-		// assert forall i, j :: 0 <= i < j < maxPriority ==> queues[i].elements != queues[j].elements;
 	}
 
 	predicate Valid()
@@ -226,15 +146,6 @@ class {:autocontracts} PriorityQueue
 		queues[queueIndex].push(value);
 		sequences := addTo(sequences, priority, value);
 		elements := elements + 1;
-		// assert |sequences| == maxPriority;
-		// assert queues.Length == maxPriority;
-		// assert elements == |flatten(sequences)|;
-		// assert (forall i :: 0 <= i < maxPriority ==> queues[i].Valid());
-		// assert (forall i, j :: 0 <= i < j < maxPriority ==> queues[i] != queues[j]);
-		// assert (forall i, j :: 0 <= i < j < maxPriority ==> queues[i].elements != queues[j].elements);
-		// assert (forall i, j :: 0 <= i < j < maxPriority ==> queues[i].Repr * queues[j].Repr == {});
-		// assert (forall i :: 0 <= i < maxPriority ==> sequences[i] == queues[i].elemSeq);
-		// assert Valid();
 	}
 
 	method pop() returns (result : Signal)
@@ -285,12 +196,16 @@ method TestPriorityQueue()
 	q.push(Brake(2), 1);
 	q.push(Beam(20), 3);
 	q.push(Brake(5), 2);
+
 	var y := q.pop();
 	assert y == Brake(2);
+
 	y := q.peek();
 	assert y == Brake(5);
+
 	y := q.pop();
 	assert y == Brake(5);
+
 	y := q.pop();
 	assert y == Beam(20);
 }
