source/Utils.dfy
@@ -1,0 +1,88 @@
+function emptyLists<T>(size : nat) : seq<seq<T>>
+	ensures |emptyLists<T>(size)| == size
+	ensures forall i :: 0 <= i < size ==> emptyLists<T>(size)[i] == []
+	ensures flatten<T>(emptyLists<T>(size)) == []
+{
+	if size == 0 then
+		[]
+	else
+		[[]] + emptyLists(size - 1)
+}
+
+function flatten<T>(sequences : seq<seq<T>>) : seq<T>
+{
+	if |sequences| == 0 then
+		[]
+	else
+		sequences[0] + flatten(sequences[1..])
+}
+
+function firstNonEmpty<T>(sequences : seq<seq<T>>) : nat
+	requires flatten<T>(sequences) != []
+	ensures 0 <= firstNonEmpty<T>(sequences) < |sequences|
+	ensures |sequences[firstNonEmpty<T>(sequences)]| > 0
+	ensures forall k :: 0 <= k < |sequences| && sequences[k] != []
+	==> firstNonEmpty<T>(sequences) <= k
+{
+	if sequences[0] != [] then
+		0
+	else
+		1 + firstNonEmpty(sequences[1..])
+}
+
+function addTo<T>(sequences : seq<seq<T>>, priority : nat, value : T) : seq<seq<T>>
+	requires 0 < priority <= |sequences|
+	ensures |addTo(sequences, priority, value)| == |sequences|
+	ensures |flatten(addTo(sequences, priority, value))| == |flatten(sequences)| + 1
+	ensures forall i :: 0 <= i < |sequences| && i != index(priority) ==> addTo(sequences, priority, value)[i] == sequences[i]
+	ensures addTo(sequences, priority, value)[index(priority)] == sequences[index(priority)] + [value] 
+{
+	var changeIndex := index(priority);
+	if changeIndex == 0 then
+		[sequences[0] + [value]] + sequences[1..]
+	else
+		[sequences[0]] + addTo(sequences[1..], priority - 1, value)
+}
+
+function removeFrom<T>(sequences : seq<seq<T>>, priority : nat) : seq<seq<T>>
+	requires 0 < priority <= |sequences|
+	requires |sequences[index(priority)]| > 0 
+	ensures |removeFrom(sequences, priority)| == |sequences|
+	ensures |flatten(removeFrom(sequences, priority))| == |flatten(sequences)| - 1
+	ensures forall i :: 0 <= i < |sequences| && i != index(priority) ==> removeFrom(sequences, priority)[i] == sequences[i]
+	ensures removeFrom(sequences, priority)[index(priority)] == sequences[index(priority)][1..]
+{
+	var changeIndex := index(priority);
+	if changeIndex == 0 then
+		[sequences[0][1..]] + sequences[1..]
+	else
+		[sequences[0]] + removeFrom(sequences[1..], priority - 1)
+}
+
+function method index(priority : nat) : nat
+	requires 0 < priority
+	ensures 0 <= index(priority)
+{
+	priority - 1
+}
+
+function priority(index : nat) : nat
+	ensures 0 < priority(index)
+{
+	index + 1
+}
+
+lemma flattenEmptyImpliesAllEmpty<T>(sequences : seq<seq<T>>)
+  ensures (|flatten(sequences)| == 0) <==>
+	  (forall i :: 0 <= i < |sequences| ==> sequences[i] == [])
+{
+	if (|flatten(sequences)| == 0) {
+		assert flatten(sequences) == [];
+		if |sequences| == 0 {
+			assert forall i :: 0 <= i < |sequences| ==> sequences[i] == [];
+		} else {
+			assert sequences[0] == [];
+			flattenEmptyImpliesAllEmpty(sequences[1..]);
+		}
+	}
+}
